refactor

Logic/Predicate/FirstOrder/Formula.lean
@@ -1,19 +1,9 @@
-import Logic.Vorspiel.Vorspiel
+import Logic.Predicate.Term
 import Mathlib.Data.Finset.Basic
 
-structure Language where
-  func : Nat → Type u
-  rel  : Nat → Type u
+namespace FirstOrder
 
 variable (L : Language.{u})
-
-inductive SubTerm (μ : Type v) (n : ℕ)
-  | fixedVar : Fin n → SubTerm μ n
-  | freeVar  : μ → SubTerm μ n
-  | func : ∀ {k}, L.func k → (Fin k → SubTerm μ n) → SubTerm μ n
-
-prefix:max "&" => SubTerm.freeVar
-prefix:max "#" => SubTerm.fixedVar
 
 inductive SubFormula (μ : Type v) : ℕ → Type (max u v) where
   | verum  {n} : SubFormula μ n
@@ -27,41 +17,15 @@ inductive SubFormula (μ : Type v) : ℕ → Type (max u v) where
 
 variable (μ : Type v) (μ₁ : Type v₁) (μ₂ : Type v₂) (μ₃ : Type v₃)
 
-@[reducible] def Term := SubFormula L μ 0
-
 @[reducible] def Formula := SubFormula L μ 0
 
 @[reducible] def Sentence := Formula L Empty
-
--- Syntactic ... : 証明で使用する項と論理式
-@[reducible] def SyntacticSubTerm (n : ℕ) := SubTerm L ℕ n
-
-@[reducible] def SyntacticTerm := SyntacticSubTerm L 0
 
 @[reducible] def SyntacticSubFormula (n : ℕ) := SubFormula L ℕ n
 
 @[reducible] def SyntacticFormula := SyntacticSubFormula L 0
 
 variable {L μ μ₁ μ₂ μ₃}
-
-namespace SubTerm
-
-variable (L)
-
-@[reducible] def func! (k) (f : L.func k) (v : Fin k → SubTerm L μ n) := func f v
-
-variable {L}
-
-variable [∀ k, ToString (L.func k)] [∀ k, ToString (L.rel k)] [ToString μ]
-
-def toStr : SubTerm L μ n → String
-  | #x       => "x_{" ++ toString (n - 1 - (x : ℕ)) ++ "}"
-  | &x       => "z_{" ++ toString x ++ "}"
-  | func f v => "{" ++ toString f ++ "} \\left(" ++ String.funFin_toStr (fun i => toStr (v i)) ++ "\\right)"
-
-instance : ToString (SubTerm L μ n) := ⟨toStr⟩
-
-end SubTerm
 
 namespace SubFormula
 variable {n n₁ n₂ : ℕ}
@@ -177,112 +141,6 @@ instance : ToString (SubFormula L μ n) := ⟨toStr⟩
 
 end SubFormula
 
-namespace SubTerm
-variable {n n₁ n₂ n₃ m m₁ m₂ m₃ : ℕ}
-
-def bind (fixed : Fin n₁ → SubTerm L μ₂ n₂) (free : μ₁ → SubTerm L μ₂ n₂) :
-    SubTerm L μ₁ n₁ → SubTerm L μ₂ n₂
-  | (#x)       => fixed x    
-  | (&x)       => free x
-  | (func f v) => func f (fun i => (v i).bind fixed free)
-
-def map (fixed : Fin n₁ → Fin n₂) (free : μ₁ → μ₂) : SubTerm L μ₁ n₁ → SubTerm L μ₂ n₂ :=
-  bind (fun n => #(fixed n)) (fun m => &(free m))
-
-def subst (t : SubTerm L μ n) : SubTerm L μ (n + 1) →  SubTerm L μ n :=
-  bind (fixedVar <: t) freeVar
-
-def fixedSucc : SubTerm L μ n → SubTerm L μ (n + 1) :=
-  map Fin.succ id
-
-section bind
-variable (fixed : Fin n₁ → SubTerm L μ₂ n₂) (free : μ₁ → SubTerm L μ₂ n₂)
-
-@[simp] lemma bind_freeVar (m : μ₁) : (&m : SubTerm L μ₁ n₁).bind fixed free = free m := rfl
-
-@[simp] lemma bind_fixedVar (n : Fin n₁) : (#n : SubTerm L μ₁ n₁).bind fixed free = fixed n := rfl
-
-@[simp] lemma bind_function {k} (f : L.func k) (v : Fin k → SubTerm L μ₁ n₁) :
-    (func f v).bind fixed free = func f (fun i => (v i).bind fixed free) := rfl
-
-end bind
-
-lemma bind_bind
-  (fixed₁ : Fin n₁ → SubTerm L μ₂ n₂) (free₁ : μ₁ → SubTerm L μ₂ n₂)
-  (fixed₂ : Fin n₂ → SubTerm L μ₃ n₃) (free₂ : μ₂ → SubTerm L μ₃ n₃) (t : SubTerm L μ₁ n₁) :
-    (t.bind fixed₁ free₁).bind fixed₂ free₂ = t.bind (fun n => (fixed₁ n).bind fixed₂ free₂) (fun m => (free₁ m).bind fixed₂ free₂) :=
-  by induction t <;> simp[*]
-
-section map
-variable (fixed : Fin n₁ → Fin n₂) (free : μ₁ → μ₂)
-
-@[simp] lemma map_freeVar (m : μ₁) : (&m : SubTerm L μ₁ n₁).map fixed free = &(free m) := rfl
-
-@[simp] lemma map_fixedVar (n : Fin n₁) : (#n : SubTerm L μ₁ n₁).map fixed free = #(fixed n) := rfl
-
-@[simp] lemma map_function {k} (f : L.func k) (v : Fin k → SubTerm L μ₁ n₁) :
-    (func f v).map fixed free = func f (fun i => (v i).map fixed free) := rfl
-
-lemma map_map
-  (fixed₁ : Fin n₁ → Fin n₂) (free₁ : μ₁ → μ₂)
-  (fixed₂ : Fin n₂ → Fin n₃) (free₂ : μ₂ → μ₃) (t : SubTerm L μ₁ n₁) :
-    (t.map fixed₁ free₁).map fixed₂ free₂ = t.map (fixed₂ ∘ fixed₁) (free₂ ∘ free₁) :=
-  bind_bind _ _ _ _ _
-
-end map
-
-@[simp] lemma fixedSucc_fixedVar (x : Fin n) : fixedSucc (#x : SubTerm L μ n) = #(Fin.succ x) := rfl
-
-@[simp] lemma fixedSucc_freeVar (x : μ) : fixedSucc (&x : SubTerm L μ n) = &x := rfl
-
-section syntactic
-
-/-
-  #0 #1 ... #(n - 1) &0 &1 ...
-   ↓shift
-  #0 #1 ... #(n - 1) &1 &2 &3 ...
--/
-
-def shift : SyntacticSubTerm L n → SyntacticSubTerm L n :=
-  map id Nat.succ
-
-def shift_le (s : ℕ) : SyntacticSubTerm L n → SyntacticSubTerm L n :=
-  map id (fun m => m + s)
-
-/- 
-  #0 #1 ... #(n - 1) #n &0 &1 ...
-   ↓push           ↑pull
-  #0 #1 ... #(n - 1) &0 &1 &2 ...
- -/
-
-def push : SyntacticSubTerm L (n + 1) → SyntacticSubTerm L n :=
-  bind (fixedVar <: &0) (fun m => &(Nat.succ m))
-
-def pull : SyntacticSubTerm L n → SyntacticSubTerm L (n + 1) :=
-  bind (fun x => #(Fin.castSucc x)) (fun x => match x with | 0 => #(Fin.last n) | x + 1 => &x)
-
-@[simp] lemma push_fixedVar_castSucc (x : Fin n) : push (#(Fin.castSucc x) : SyntacticSubTerm L (n + 1)) = #x := by simp[push]
-
-@[simp] lemma push_fixedVar_last : push (#(Fin.last n) : SyntacticSubTerm L (n + 1)) = &0 := by simp[push]
-
-@[simp] lemma push_freeVar (x : ℕ) : push (&x : SyntacticSubTerm L (n + 1)) = &(x + 1) := by simp[push]
-
-@[simp] lemma push_function {k} (f : L.func k) (v : Fin k → SyntacticSubTerm L (n + 1)) :
-    push (func f v) = func f (fun i => push $ v i) := by simp[push]
-
-@[simp] lemma pull_fixedVar (x : Fin n) : pull (#x : SyntacticSubTerm L n) = #(Fin.castSucc x) := by simp[pull]
-
-@[simp] lemma pull_freeVar_zero : pull (&0 : SyntacticSubTerm L n) = #(Fin.last n) := by simp[pull]
-
-@[simp] lemma pull_freeVar_succ (x : ℕ) : pull (&(x + 1) : SyntacticSubTerm L n) = &x := by simp[pull]
-
-@[simp] lemma pull_function {k} (f : L.func k) (v : Fin k → SyntacticSubTerm L n) :
-    pull (func f v) = func f (fun i => pull $ v i) := by simp[pull]
-
-end syntactic
-
-end SubTerm
-
 namespace SubFormula
 variable {n n₁ n₂ n₃ m m₁ m₂ m₃ : ℕ}
 
@@ -391,7 +249,7 @@ lemma map_map
     map fixed₂ free₂ (map fixed₁ free₁ p) = map (fixed₂ ∘ fixed₁) (free₂ ∘ free₁) p :=
   bind_bind _ _ _ _ _
 
-section syntactic
+section Syntactic
 
 def shift : SyntacticSubFormula L n →L SyntacticSubFormula L n :=
   map id Nat.succ
@@ -446,6 +304,12 @@ def pull : SyntacticSubFormula L n →L SyntacticSubFormula L (n + 1) :=
   · exact funext (Fin.cases (by simp) (by simp[Fin.succ_castSucc])) 
   · exact funext (Nat.rec (by simp) (by simp))
 
-end syntactic
+end Syntactic
 
 end SubFormula
+
+@[reducible] def Theory (L : Language) (μ) := Set (Formula L μ)
+
+@[reducible] def CTheory (L : Language) := Set (Sentence L)
+
+end FirstOrder
