Logic/Predicate/FirstOrder/Language.lean
@@ -1,0 +1,83 @@
+import Logic.Predicate.FirstOrder.Formula
+
+variable {L L₁ L₂ L₃ : Language} {μ : Type _}
+
+namespace Language
+
+namespace Hom
+variable (Φ : Hom L₁ L₂) {n : ℕ}
+
+open FirstOrder
+
+def onFOFormula' (Φ : Hom L₁ L₂) : ∀ {n}, SubFormula L₁ μ n → SubFormula L₂ μ n
+  | _, ⊤                   => ⊤ 
+  | _, ⊥                   => ⊥ 
+  | _, SubFormula.rel r v  => SubFormula.rel (Φ.onRel r) (fun i => Φ.onTerm (v i))
+  | _, SubFormula.nrel r v => SubFormula.nrel (Φ.onRel r) (fun i => Φ.onTerm (v i))
+  | _, p ⋏ q               => Φ.onFOFormula' p ⋏ Φ.onFOFormula' q
+  | _, p ⋎ q               => Φ.onFOFormula' p ⋎ Φ.onFOFormula' q
+  | _, ∀' p                => ∀' Φ.onFOFormula' p
+  | _, ∃' p                => ∃' Φ.onFOFormula' p
+
+lemma onFOFormula'_neg {n} (p : SubFormula L₁ μ n) :
+    Φ.onFOFormula' (¬'p) = ¬' Φ.onFOFormula' p :=
+  by induction p using SubFormula.rec' <;> simp[*, onFOFormula', ←SubFormula.neg_eq]
+
+def onFOFormula (Φ : Hom L₁ L₂) {n} : SubFormula L₁ μ n →L SubFormula L₂ μ n where
+  toFun := Φ.onFOFormula'
+  map_top' := by simp[onFOFormula']
+  map_bot' := by simp[onFOFormula']
+  map_and' := by simp[onFOFormula']
+  map_or'  := by simp[onFOFormula']
+  map_neg' := by simp[onFOFormula'_neg]
+  map_imp' := by simp[SubFormula.imp_eq, onFOFormula'_neg, ←SubFormula.neg_eq, onFOFormula']
+
+@[simp] lemma onFOFormula_rel {k} (r : L₁.rel k) (v : Fin k → SubTerm L₁ μ n) :
+    Φ.onFOFormula (SubFormula.rel r v) = SubFormula.rel (Φ.onRel r) (fun i => Φ.onTerm (v i)) := rfl
+
+lemma onFOFormula_nrel {k} (r : L₁.rel k) (v : Fin k → SubTerm L₁ μ n) :
+    Φ.onFOFormula (SubFormula.nrel r v) = SubFormula.nrel (Φ.onRel r) (fun i => Φ.onTerm (v i)) := rfl
+
+lemma onFOFormula_all (p : SubFormula L₁ μ (n + 1)) :
+    Φ.onFOFormula (∀' p) = ∀' Φ.onFOFormula p := rfl
+
+lemma onFOFormula_ex (p : SubFormula L₁ μ (n + 1)) :
+    Φ.onFOFormula (∃' p) = ∃' Φ.onFOFormula p := rfl
+
+end Hom
+
+end Language
+
+variable {L : Language} [∀ k, DecidableEq (L.func k)] [∀ k, DecidableEq (L.rel k)]
+
+namespace FirstOrder
+
+namespace SubFormula
+
+noncomputable def langf : ∀ {n}, SubFormula L μ n → Finset (Σ k, L.func k)
+  | _, ⊤        => ∅
+  | _, ⊥        => ∅
+  | _, rel  _ v => Finset.bunionᵢ Finset.univ (fun i => SubTerm.langf (v i))
+  | _, nrel _ v => Finset.bunionᵢ Finset.univ (fun i => SubTerm.langf (v i))
+  | _, p ⋏ q    => langf p ∪ langf q 
+  | _, p ⋎ q    => langf p ∪ langf q 
+  | _, ∀' p     => langf p 
+  | _, ∃' p     => langf p 
+
+noncomputable def langr : ∀ {n}, SubFormula L μ n → Finset (Σ k, L.rel k)
+  | _, ⊤        => ∅
+  | _, ⊥        => ∅
+  | _, rel  r _ => {⟨_, r⟩}
+  | _, nrel r _ => {⟨_, r⟩}
+  | _, p ⋏ q    => langr p ∪ langr q 
+  | _, p ⋎ q    => langr p ∪ langr q 
+  | _, ∀' p     => langr p 
+  | _, ∃' p     => langr p 
+
+def lang (p : SubFormula L μ n) : Language :=
+  Language.subLanguage L (fun k f => ⟨k, f⟩ ∈ langf p) (fun k r => ⟨k, r⟩ ∈ langr p) 
+
+end SubFormula
+
+end FirstOrder
+
