Logic/Predicate/Language.lean
@@ -1,0 +1,70 @@
+import Logic.Vorspiel.Vorspiel
+import Mathlib.Data.Finset.Basic
+
+structure Language where
+  func : Nat → Type u
+  rel  : Nat → Type u
+
+namespace Language
+
+protected def empty : Language.{u} where
+  func := fun _ => PEmpty
+  rel  := fun _ => PEmpty
+
+instance : Inhabited Language := ⟨Language.empty⟩
+
+inductive GraphFunc : ℕ → Type
+  | start : GraphFunc 0
+  | terminal : GraphFunc 0
+
+inductive GraphRel : ℕ → Type
+  | equal : GraphRel 2
+  | le : GraphRel 2
+
+def graph : Language where
+  func := GraphFunc
+  rel := GraphRel
+
+inductive BinaryRel : ℕ → Type
+  | isone : BinaryRel 1
+  | equal : BinaryRel 2
+  | le : BinaryRel 2
+
+def binary : Language where
+  func := fun _ => Empty
+  rel := BinaryRel
+
+inductive EqRel : ℕ → Type
+  | equal : EqRel 2
+
+def equal : Language where
+  func := fun _ => Empty
+  rel := EqRel
+
+instance (k) : ToString (equal.func k) := ⟨fun _ => ""⟩
+instance (k) : ToString (equal.rel k) := ⟨fun _ => "\\mathrm{Equal}"⟩
+
+structure Hom (L₁ L₂ : Language) where
+  onFunc : {k : ℕ} → L₁.func k → L₂.func k
+  onRel : {k : ℕ} → L₁.rel k → L₂.rel k
+
+namespace Hom
+variable (L L₁ L₂ L₃ : Language) (Φ : Hom L₁ L₂)
+
+protected def id : Hom L L where
+  onFunc := id
+  onRel := id
+
+variable {L L₁ L₂ L₃}
+
+def comp (Ψ : Hom L₂ L₃) (Φ : Hom L₁ L₂) : Hom L₁ L₃ where
+  onFunc := Ψ.onFunc ∘ Φ.onFunc 
+  onRel  := Ψ.onRel ∘ Φ.onRel 
+
+end Hom
+
+def subLanguage (L : Language) (pfunc : ∀ k, Language.func L k → Prop) (prel : ∀ k, L.rel k → Prop) : Language where
+  func := fun k => Subtype (pfunc k)
+  rel  := fun k => Subtype (prel k)
+
+end Language
