Logic/Predicate/Term.lean
@@ -1,0 +1,170 @@
+import Logic.Predicate.Language
+
+variable (L : Language.{u}) (L₁ L₂ L₃ : Language)
+
+inductive SubTerm (μ : Type v) (n : ℕ)
+  | fixedVar : Fin n → SubTerm μ n
+  | freeVar  : μ → SubTerm μ n
+  | func : ∀ {k}, L.func k → (Fin k → SubTerm μ n) → SubTerm μ n
+
+prefix:max "&" => SubTerm.freeVar
+prefix:max "#" => SubTerm.fixedVar
+
+variable (μ : Type v) (μ₁ : Type v₁) (μ₂ : Type v₂) (μ₃ : Type v₃)
+
+@[reducible] def Term := SubTerm L μ 0
+
+@[reducible] def SyntacticSubTerm (n : ℕ) := SubTerm L ℕ n
+
+@[reducible] def SyntacticTerm := SyntacticSubTerm L 0
+
+namespace SubTerm
+variable {μ μ₁ μ₂ μ₃}
+
+@[reducible] def func! (k) (f : L.func k) (v : Fin k → SubTerm L μ n) := func f v
+
+variable {L}
+
+variable [∀ k, ToString (L.func k)] [∀ k, ToString (L.rel k)] [ToString μ]
+
+def toStr : SubTerm L μ n → String
+  | #x       => "x_{" ++ toString (n - 1 - (x : ℕ)) ++ "}"
+  | &x       => "z_{" ++ toString x ++ "}"
+  | func f v => "{" ++ toString f ++ "} \\left(" ++ String.funFin_toStr (fun i => toStr (v i)) ++ "\\right)"
+
+instance : ToString (SubTerm L μ n) := ⟨toStr⟩
+
+variable {n n₁ n₂ n₃ m m₁ m₂ m₃ : ℕ}
+
+def bind (fixed : Fin n₁ → SubTerm L μ₂ n₂) (free : μ₁ → SubTerm L μ₂ n₂) :
+    SubTerm L μ₁ n₁ → SubTerm L μ₂ n₂
+  | (#x)       => fixed x    
+  | (&x)       => free x
+  | (func f v) => func f (fun i => (v i).bind fixed free)
+
+def map (fixed : Fin n₁ → Fin n₂) (free : μ₁ → μ₂) : SubTerm L μ₁ n₁ → SubTerm L μ₂ n₂ :=
+  bind (fun n => #(fixed n)) (fun m => &(free m))
+
+def subst (t : SubTerm L μ n) : SubTerm L μ (n + 1) →  SubTerm L μ n :=
+  bind (fixedVar <: t) freeVar
+
+def fixedSucc : SubTerm L μ n → SubTerm L μ (n + 1) :=
+  map Fin.succ id
+
+section bind
+variable (fixed : Fin n₁ → SubTerm L μ₂ n₂) (free : μ₁ → SubTerm L μ₂ n₂)
+
+@[simp] lemma bind_freeVar (m : μ₁) : (&m : SubTerm L μ₁ n₁).bind fixed free = free m := rfl
+
+@[simp] lemma bind_fixedVar (n : Fin n₁) : (#n : SubTerm L μ₁ n₁).bind fixed free = fixed n := rfl
+
+@[simp] lemma bind_function {k} (f : L.func k) (v : Fin k → SubTerm L μ₁ n₁) :
+    (func f v).bind fixed free = func f (fun i => (v i).bind fixed free) := rfl
+
+end bind
+
+lemma bind_bind
+  (fixed₁ : Fin n₁ → SubTerm L μ₂ n₂) (free₁ : μ₁ → SubTerm L μ₂ n₂)
+  (fixed₂ : Fin n₂ → SubTerm L μ₃ n₃) (free₂ : μ₂ → SubTerm L μ₃ n₃) (t : SubTerm L μ₁ n₁) :
+    (t.bind fixed₁ free₁).bind fixed₂ free₂ = t.bind (fun n => (fixed₁ n).bind fixed₂ free₂) (fun m => (free₁ m).bind fixed₂ free₂) :=
+  by induction t <;> simp[*]
+
+section map
+variable (fixed : Fin n₁ → Fin n₂) (free : μ₁ → μ₂)
+
+@[simp] lemma map_freeVar (m : μ₁) : (&m : SubTerm L μ₁ n₁).map fixed free = &(free m) := rfl
+
+@[simp] lemma map_fixedVar (n : Fin n₁) : (#n : SubTerm L μ₁ n₁).map fixed free = #(fixed n) := rfl
+
+@[simp] lemma map_function {k} (f : L.func k) (v : Fin k → SubTerm L μ₁ n₁) :
+    (func f v).map fixed free = func f (fun i => (v i).map fixed free) := rfl
+
+lemma map_map
+  (fixed₁ : Fin n₁ → Fin n₂) (free₁ : μ₁ → μ₂)
+  (fixed₂ : Fin n₂ → Fin n₃) (free₂ : μ₂ → μ₃) (t : SubTerm L μ₁ n₁) :
+    (t.map fixed₁ free₁).map fixed₂ free₂ = t.map (fixed₂ ∘ fixed₁) (free₂ ∘ free₁) :=
+  bind_bind _ _ _ _ _
+
+end map
+
+@[simp] lemma fixedSucc_fixedVar (x : Fin n) : fixedSucc (#x : SubTerm L μ n) = #(Fin.succ x) := rfl
+
+@[simp] lemma fixedSucc_freeVar (x : μ) : fixedSucc (&x : SubTerm L μ n) = &x := rfl
+
+section Syntactic
+
+/-
+  #0 #1 ... #(n - 1) &0 &1 ...
+   ↓shift
+  #0 #1 ... #(n - 1) &1 &2 &3 ...
+-/
+
+def shift : SyntacticSubTerm L n → SyntacticSubTerm L n :=
+  map id Nat.succ
+
+def shift_le (s : ℕ) : SyntacticSubTerm L n → SyntacticSubTerm L n :=
+  map id (fun m => m + s)
+
+/- 
+  #0 #1 ... #(n - 1) #n &0 &1 ...
+   ↓push           ↑pull
+  #0 #1 ... #(n - 1) &0 &1 &2 ...
+ -/
+
+def push : SyntacticSubTerm L (n + 1) → SyntacticSubTerm L n :=
+  bind (fixedVar <: &0) (fun m => &(Nat.succ m))
+
+def pull : SyntacticSubTerm L n → SyntacticSubTerm L (n + 1) :=
+  bind (fun x => #(Fin.castSucc x)) (#(Fin.last n) :>ₙ freeVar)
+
+@[simp] lemma push_fixedVar_castSucc (x : Fin n) : push (#(Fin.castSucc x) : SyntacticSubTerm L (n + 1)) = #x := by simp[push]
+
+@[simp] lemma push_fixedVar_last : push (#(Fin.last n) : SyntacticSubTerm L (n + 1)) = &0 := by simp[push]
+
+@[simp] lemma push_freeVar (x : ℕ) : push (&x : SyntacticSubTerm L (n + 1)) = &(x + 1) := by simp[push]
+
+@[simp] lemma push_function {k} (f : L.func k) (v : Fin k → SyntacticSubTerm L (n + 1)) :
+    push (func f v) = func f (fun i => push $ v i) := by simp[push]
+
+@[simp] lemma pull_fixedVar (x : Fin n) : pull (#x : SyntacticSubTerm L n) = #(Fin.castSucc x) := by simp[pull]
+
+@[simp] lemma pull_freeVar_zero : pull (&0 : SyntacticSubTerm L n) = #(Fin.last n) := by simp[pull]
+
+@[simp] lemma pull_freeVar_succ (x : ℕ) : pull (&(x + 1) : SyntacticSubTerm L n) = &x := by simp[pull]
+
+@[simp] lemma pull_function {k} (f : L.func k) (v : Fin k → SyntacticSubTerm L n) :
+    pull (func f v) = func f (fun i => pull $ v i) := by simp[pull]
+
+end Syntactic
+
+variable {L : Language} [∀ k, DecidableEq (L.func k)] [∀ k, DecidableEq (L.rel k)]
+
+def langf : SubTerm L μ n → Finset (Σ k, L.func k)
+  | #_       => ∅
+  | &_       => ∅
+  | func f v => insert ⟨_, f⟩ $ Finset.bunionᵢ Finset.univ (fun i => langf (v i))
+
+end SubTerm
+
+namespace Language
+
+namespace Hom
+variable {L L₁ L₂ L₃} {μ} (Φ : Hom L₁ L₂)
+
+def onTerm (Φ : Hom L₁ L₂) : SubTerm L₁ μ n → SubTerm L₂ μ n
+  | #x               => #x
+  | &x               => &x
+  | SubTerm.func f v => SubTerm.func (Φ.onFunc f) (fun i => onTerm Φ (v i))
+
+@[simp] lemma onTerm_fixedVar (x : Fin n) : Φ.onTerm (#x : SubTerm L₁ μ n) = #x := rfl
+
+@[simp] lemma onTerm_freeVar (x : μ) : Φ.onTerm (&x : SubTerm L₁ μ n) = &x := rfl
+
+@[simp] lemma onTerm_func {k} (f : L₁.func k) (v : Fin k → SubTerm L₁ μ n) :
+    Φ.onTerm (SubTerm.func f v) = SubTerm.func (Φ.onFunc f) (fun i => onTerm Φ (v i)) := rfl
+
+end Hom
+
+end Language
+
+
